LambdaS5/coq/LjsSyntax.v
@@ -1,7 +1,7 @@
+Require Import JsNumber.
 Require Import LjsShared.
 Require Import Utils.
 Require Import String.
-Require Import JsNumber.
 Require Import Coq.Strings.String.
 Require LibStream.
 
@@ -176,7 +176,7 @@ Fixpoint expr_fv e : finset id := match e with
 | expr_try_catch e1 e2 => expr_fv e1 \u expr_fv e2
 | expr_try_finally e1 e2 => expr_fv e1 \u expr_fv e2
 | expr_throw e => expr_fv e
-| expr_lambda is e => expr_fv e \- FinsetImpl.from_list is
+| expr_lambda is e => expr_fv e \- from_list is
 | expr_eval e1 e2 => expr_fv e1 \u expr_fv e2
 | expr_hint _ e => expr_fv e
 end
